src/Auto.v
@@ -1,0 +1,87 @@
+Require Import GenStMonad StructTactics MonadVM.
+Require Import Coq.Arith.Peano_dec.
+
+Ltac fail_if_in_hyps H := 
+  let t := type of H in 
+  lazymatch goal with 
+  | [G : t |- _ ] => fail "There is already a hypothesis of this proof"
+  | [_ : _ |- _ ] => idtac
+  end.
+
+Ltac pose_new_proof H := 
+  fail_if_in_hyps H;
+  pose proof H.
+
+Ltac fail_if_in_hyps_type t := 
+  lazymatch goal with 
+  | [G : t |- _ ] => fail "There is already a hypothesis of this type"
+  | [_ : _ |- _ ] => idtac
+  end.
+
+Ltac assert_new_proof_by H tac := 
+  fail_if_in_hyps_type H;
+  assert H by tac.
+
+Ltac jkjk :=
+  match goal with
+  | [H: context[?X] |- ?X = _] => rewrite H
+  end.
+
+Ltac jkjk' :=
+  match goal with
+  | H: _ |- _ => rewrite H; reflexivity
+  end.
+
+Ltac dunit :=
+  match goal with
+  | [H:unit |- _] => destruct H
+  end.
+
+Ltac dohtac := (*try htac; *)
+               try rewrite PeanoNat.Nat.eqb_refl in *;
+               try rewrite PeanoNat.Nat.eqb_eq in *.
+
+
+Ltac df :=
+  repeat (
+      cbn in *;
+      unfold runSt in *;
+      repeat break_let;
+      repeat (monad_unfold; cbn in *; find_inversion);
+      monad_unfold;
+      repeat dunit;
+      unfold snd in * ).
+
+Ltac dosome :=
+  repeat (
+      match goal with
+      | [H: match ?o with
+            | Some _ => _
+            | _ => _
+            end
+            =
+            (Some _, _) |- _] =>
+        destruct o; try solve_by_inversion
+      end; df).
+
+Ltac subst' :=
+  match goal with
+  | [H: ?A = _, H2: context[?A] |- _] => rewrite H in *; clear H
+  | [H: ?A = _ |- context[?A]] => rewrite H in *; clear H
+  end.
+
+Ltac subst'' :=
+  match goal with
+  | [H:?A = _, H2: context [?A] |- _] => rewrite H in *
+  | [H:?A = _ |- context [?A]] => rewrite H in *
+  end.
+
+Ltac dooit :=
+  repeat eexists;
+  cbn;
+  repeat break_let;
+  simpl;
+  repeat find_inversion;
+  subst';
+  df;
+  reflexivity.
