src/AutoApp.v
@@ -1,0 +1,117 @@
+Require Import StructTactics Auto VmSemantics StVM MonadVM GenStMonad.
+Require Import List.
+
+Ltac dosome :=
+  repeat (
+      match goal with
+      | [H: match ?o with
+            | Some _ => _
+            | _ => _
+            end
+            =
+            (Some _, _) |- _] =>
+        destruct o; try solve_by_inversion
+      end; df).
+
+Ltac tacc H :=
+  (symmetry;
+   erewrite <- pl_immut in *;
+   rewrite H;
+   eauto ).
+
+Ltac ff := repeat break_match; try solve_by_inversion; df.
+
+Ltac dosome_eq y :=
+  match goal with
+  | [H: match ?x with _ => _ end = (Some _, _)  |- _] =>
+    destruct x eqn:y; try solve_by_inversion
+  end.
+
+Ltac do_pair :=
+  match goal with
+  | [H: (_,_) = (Some _,_) |- _] => invc H
+  | [H: (Some _,_) = (_,_) |- _] => invc H
+  end.
+
+Ltac dosome_eqj :=
+  let y := fresh in 
+  match goal with
+  | [H: match ?x with _ => _ end = (Some _, _)  |- _] =>
+    destruct x eqn:y; try solve_by_inversion
+  end.
+
+Ltac dosome'' :=
+  match goal with
+  | [H: (_,_) = (Some _, _) |- _] => invc H
+  end.
+
+Ltac domap :=
+  let n := fresh in
+  match goal with
+  | [H: match ?X with _ => _ end _ = (Some _, _) |- _] =>
+    destruct X eqn:n; try solve_by_inversion
+  end.
+
+
+Ltac doit' := repeat dosome_eqj;
+              repeat break_let;
+              repeat do_pair;
+              repeat break_let;
+              repeat do_pair;
+              repeat dosome''.
+
+Ltac doit := repeat doit'.
+
+(*
+  Ltac map_get_subst :=
+  match goal with
+  | [H: map_get ?A ?B = _,
+  H2: context[map_get ?A ?B] |- _] =>
+  rewrite H in *; clear H
+  end.
+ *)
+
+Ltac haaa :=
+  let x:= fresh in
+  match goal with
+  | [H: context[match ?ee with | Some _ => _ | _ => _ end] |- _] =>
+    destruct ee eqn:x;
+    try solve_by_inversion
+  end; df; eauto.
+
+Ltac stt :=
+  cbn in *;
+  monad_unfold;
+  try solve_by_inversion;
+  repeat break_let;
+  dosome;
+  try haaa.
+
+Ltac dosome_eq' y :=
+  match goal with
+  | H:match ?x with
+      | _ => _
+      end _ = (Some _, _) |- _ => destruct x eqn:y; try solve_by_inversion
+  end.
+
+Ltac dothat :=
+  unfold StVM.st_ev, StVM.st_pl, StVM.st_trace, StVM.st_store in *;
+  try unfold st_ev in *;
+  try unfold st_pl in *;
+  try unfold st_trace in *;
+  try unfold st_store in *.
+
+Ltac ff' :=
+  repeat break_match; try solve_by_inversion.
+
+Ltac do_inv_head :=
+  let tac := (eapply app_inv_head; eauto) in
+  repeat
+    match goal with
+    | [H: ?ls ++ ?xs = ?ls ++ ?ys |- _] => assert_new_proof_by (xs = ys) tac
+    end.
+
+Ltac doex := 
+  unfold extractUev, extractSig in *;
+  ff';
+  unfold ret in *; doit.
