src/Axioms_Io.v
@@ -1,0 +1,37 @@
+Require Import Term ConcreteEvidence.
+
+(** IO Axioms *)
+
+Definition remote_events (t:AnnoTerm) (p:Plc) : (list Ev).
+Admitted.
+Definition toRemote (t:Term) (*(pTo:Plc)*) (e:EvidenceC) : EvidenceC.
+Admitted.
+Definition parallel_eval_thread (t:Term) (e:EvidenceC) : EvidenceC.
+Admitted.
+
+Definition parallel_att_vm_thread (t:AnnoTerm) (e:EvidenceC) : EvidenceC.
+Admitted.
+
+Definition parallel_vm_events (t:AnnoTerm) (p:Plc) : list Ev.
+Admitted.
+
+Definition shuffled_events (el1:list Ev) (el2:list Ev) : list Ev.
+Admitted.
+
+Definition remote_evidence (t:AnnoTerm) (e:EvidenceC) : EvidenceC.
+Admitted.
+
+Definition remote_trace (t:AnnoTerm) (p:Plc) : list Ev.
+Admitted.
+
+Axiom at_evidence : forall t e,
+    toRemote (unanno t) e = remote_evidence t e.
+
+Axiom at_events : forall t p,
+  remote_events t p = remote_trace t p.
+
+Axiom par_evidence : forall t e,
+    parallel_att_vm_thread t e = remote_evidence t e.
+
+Axiom par_events : forall t p,
+  parallel_vm_events t p = remote_trace t p.
