src/MonadVM.v
@@ -4,7 +4,7 @@ Definition of the AVM Monad + monadic helper functions.
 Author:  Adam Petz, ampetz@ku.edu
 *)
 
-Require Import Term ConcreteEvidence GenStMonad.
+Require Import Term ConcreteEvidence GenStMonad Axioms_Io.
 Require Import Maps.
 
 Require Import List.
@@ -14,67 +14,10 @@ Require Import StructTactics.
 
 Require Export StVM.
 
-Print vm_st.
-
-
 Definition VM := St vm_st.
-(*Definition runVM{A:Type} := @runSt vm_config A.*)
 
-(* Sanity checks *)
-
-Definition fail_early : VM EvidenceC :=
-  ret mtc ;;
-  put (mk_st (ggc 3 mtc) [] 0 []) ;;
-  failm (A:=nat) ;;
-  put (mk_st (ggc 4 mtc) [] 0 []) ;;
-  failm (A:=nat) ;;
-  ret (ggc 3 mtc).
-
-Compute (runSt (mk_st mtc [] 0 []) fail_early).
-
-
-(*
-Definition extractVal (r:vm_st) : nat :=
-  let ev := head (st_stack r) in
-  let n :=
-      match ev with
-        | Some (ggc n _) => n
-        | _ => 0
-      end in
-  n + 1.
-
-Definition test_comp : VM unit :=
-  v <- get ;;
-    let n := extractVal v in
-    put (mk_st mtc [(ggc n mtc)] [] 0 []) ;;
-        ret tt.
-
-Definition empty_vm_state := mk_st mtc  [] 0 [].
-
-Compute (runSt empty_vm_state test_comp).
-*)
 
 (* VM monad operations *)
-
-(*
-Definition push_stackm (e:EvidenceC) : VM unit :=
-  st <- get ;;
-     let '{| st_ev := oldEv; st_stack := oldStack; st_trace := tr; st_pl := oldP; st_store := oldStore |} := st in
-     let newStack := push_stack _ e oldStack in
-     put (mk_st oldEv newStack tr oldP oldStore).
-
-Definition pop_stackm : VM EvidenceC :=
-  st <- get ;;
-     let '{| st_ev := oldE; st_stack := oldStack; st_trace := tr; st_pl := oldP; st_store := oldStore |} := st in
-     (*let oldStack := st_stack st in*)
-     let maybePopped := pop_stack _ oldStack in
-     match maybePopped with
-     | Some (e,s') =>
-       put (mk_st oldE s' tr oldP oldStore) ;;
-           ret e
-     | None => failm
-     end.
-*)
 
 Definition put_store (n:nat) (e:EvidenceC) : VM unit :=
   st <- get ;;
@@ -130,15 +73,7 @@ Definition split_evm (i:nat) (sp1 sp2:SP) (e:EvidenceC) (p:Plc) : VM (EvidenceC*
                ret (e1,e2).
 *)
 
-(** * Place-holder axioms for IO operations *)
-(* Definition invokeKIM (i:ASP_ID) (q:Plc) (*(args:list Arg)*) : BS. 
-Admitted. *)
-Print BS.
-(*
-Definition BS_res : BS.
-Admitted. *)
-
-Check put_ev.
+(** * Partially-symbolic implementations of IO operations *)
 
 Definition invokeUSM (x:nat) (i:ASP_ID) (l:list Arg) (e:EvidenceC) : VM BS :=
   (*e <- get_ev ;; *)
@@ -164,51 +99,10 @@ Definition hashEv (x:nat) (p:Plc) : VM EvidenceC :=
   ret (hhc x e).
 *)
 
-
-
 Definition copyEv (x:nat) : VM EvidenceC :=
   p <- get_pl ;;
   add_tracem [Term.copy x p] ;;
   get_ev.
-
-
-Definition remote_events (t:AnnoTerm) (p:Plc) : (list Ev).
-Admitted.
-
-Definition toRemote (t:Term) (*(pTo:Plc)*) (e:EvidenceC) : EvidenceC.
-Admitted.
-Definition parallel_eval_thread (t:Term) (e:EvidenceC) : EvidenceC.
-Admitted.
-
-Definition sendReq (reqi:nat) (q:Plc) (t:AnnoTerm) : VM unit :=
-  p <- get_pl ;;
-  add_tracem [req reqi p q (unanno t)].
-
-Definition doRemote (t:AnnoTerm) (q:Plc) (e:EvidenceC) (rpyi:nat) : VM unit :=
-  add_tracem (remote_events t q) ;;
-  put_store rpyi (toRemote (unanno t) e).
-
-Definition receiveResp (rpyi:nat) (q:Plc) : VM EvidenceC :=
-  e <- get_store_at rpyi ;;
-  p <- get_pl ;;
-  add_tracem [rpy (Nat.pred rpyi) p q] ;;
-  ret e.
-
-Require Import VM_IO_Axioms.
-
-Definition runParThread (t:AnnoTerm) (p:Plc) (e:EvidenceC) : VM (list Ev) :=
-  let el := parallel_vm_events t p in
-  let e' := parallel_att_vm_thread t e in
-  let loc := fst (range t) in
-  put_store loc e' ;;
-  ret el.
-
-Definition runParThreads (t1 t2:AnnoTerm) (p:Plc) (e1 e2:EvidenceC) : VM unit :=
-  el1 <- runParThread t1 p e1 ;;
-  el2 <- runParThread t2 p e2 ;;
-  add_tracem (shuffled_events el1 el2).
-
-
 
 Definition do_prim (x:nat) (a:ASP) : VM EvidenceC :=
   match a with
@@ -225,8 +119,104 @@ Definition do_prim (x:nat) (a:ASP) : VM EvidenceC :=
  (* | HSH => hashEv x p  *)
   end.
 
+Definition sendReq (reqi:nat) (q:Plc) (t:AnnoTerm) : VM unit :=
+  p <- get_pl ;;
+  add_tracem [req reqi p q (unanno t)].
+
+Definition receiveResp (rpyi:nat) (q:Plc) : VM EvidenceC :=
+  e <- get_store_at rpyi ;;
+  p <- get_pl ;;
+  add_tracem [rpy (Nat.pred rpyi) p q] ;;
+  ret e.
+
+(* Primitive VM Monad operations that require IO Axioms *)
+Definition doRemote (t:AnnoTerm) (q:Plc) (e:EvidenceC) (rpyi:nat) : VM unit :=
+  add_tracem (remote_events t q) ;;
+  put_store rpyi (toRemote (unanno t) e).
+
+Definition runParThread (t:AnnoTerm) (p:Plc) (e:EvidenceC) : VM (list Ev) :=
+  let el := parallel_vm_events t p in
+  let e' := parallel_att_vm_thread t e in
+  let loc := fst (range t) in
+  put_store loc e' ;;
+  ret el.
+
+Definition runParThreads (t1 t2:AnnoTerm) (p:Plc) (e1 e2:EvidenceC) : VM unit :=
+  el1 <- runParThread t1 p e1 ;;
+  el2 <- runParThread t2 p e2 ;;
+  add_tracem (shuffled_events el1 el2).
+
+(** * Helper functions for Appraisal *)
+
+Definition extractUev (e:EvidenceC) : VM (BS * EvidenceC) :=
+  match e with
+  | uuc i bs e' => ret (bs,e')
+  | _ => failm
+  end.
+
+Definition extractSig (e:EvidenceC) : VM (BS * EvidenceC) :=
+  match e with
+  | ggc bs e' => ret (bs, e')
+  | _ => failm
+  end.
+
+(*
+Definition extractHsh (e:EvidenceC) : VM (BS * EvidenceC) :=
+  match e with
+  | hhc bs e' => ret (bs, e')
+  | _ => failm
+  end. *)
+
+(*
+Definition extractComp (e:EvidenceC) : VM (EvidenceC * EvidenceC) :=
+  match e with
+  | ssc e1 e2 => ret (e1,e2)
+  | ppc e1 e2 => ret (e1,e2)
+  | _ => failm
+  end.
+ *)
+
+Definition checkSig (x:nat) (i:ASP_ID) (e':EvidenceC) (sig:BS) : VM BS :=
+  invokeUSM x i ([encodeEv e'] ++ [sig] (* ++ args*) ) mtc.
+
+Definition checkUSM (x:nat) (i:ASP_ID) (l:list Arg) (bs:BS) : VM BS :=
+  invokeUSM x i ([bs] ++ l) mtc.
+   
+Ltac monad_unfold :=
+  repeat unfold
+  execSt,  
+  do_prim,
+  invokeUSM,
+  signEv,
+  (*hashEv, *)
+  copyEv,
+
+  sendReq,
+  doRemote,
+  receiveResp,
+
+  get_ev,
+  get_pl,
+  add_tracem,
+  modify_evm,
+  (*split_evm,*)
+  add_trace,
+  failm,
+  (* Uncommenting these evaluates too much, can't apply lemmas *)
+  (*get_store_at,*)
+  get,
+  when,
+  put,
+  nop,
+  modify,
+  bind,
+  ret in *;
+  simpl in *.
 
 
+
+
+(*
 Definition eval_asp (a:ASP) (e:EvidenceC) : EvidenceC :=
   match a with
   | CPY => e 
@@ -358,39 +348,4 @@ Proof.
       destruct s; destruct s0; simpl in *; subst;
         econstructor; (try simpl); eauto; try (econstructor) . *)
 Defined.
-      
-Ltac monad_unfold :=
-  repeat unfold
-  execSt,  
-  do_prim,
-  invokeUSM,
-  signEv,
-  (*hashEv, *) (*
-  copyEv, *)
-
-  sendReq,
-  doRemote,
-  receiveResp,
-
-  
-  get_ev,
-  get_pl,
-  add_tracem,
-  modify_evm,
-  (*split_evm,*)
-  add_trace,
-  failm,
-  (* Uncommenting these evaluates too much, can't apply lemmas *)
-  (*push_stackm,
-  pop_stackm, *)
-  (*push_stack,
-  pop_stack, *)
-  (*get_store_at,*)
-  get,
-  when,
-  put,
-  nop,
-  modify,
-  bind,
-  ret in *;
-  simpl in *.
+*)
